pcuic/theories/TemplateToPCUICExpanded.v
@@ -1,3 +1,4 @@
+From Equations Require Import Equations.
 From Coq Require Import ssreflect.
 From MetaCoq.Template Require Import config utils.
 From MetaCoq.Template Require Ast TypingWf WfAst TermEquality EtaExpand.
@@ -10,16 +11,183 @@ Tactic Notation "wf_inv" ident(H) simple_intropattern(p) :=
 (eapply WfAst.wf_inv in H; progress cbn in H; try destruct H as p) || 
 (apply WfAst.wf_mkApps_napp in H; [|easy]; try destruct H as p).
 
-
 Local Hint Constructors expanded : expanded.
+
+Lemma expanded_context_map2_bias_left Σ n bctx ctx :
+  #|ctx| = #|bctx| ->
+  expanded_context Σ n ctx ->
+  expanded_context Σ n
+     (map2_bias_left set_binder_name dummy_decl bctx ctx).
+Proof.
+  unfold expanded_context.
+  intros hl. 
+  rewrite map2_map2_bias_left //.
+  intros [a]. sq.
+  induction a in bctx, hl |- *; try econstructor; auto.
+  - cbn. destruct bctx; constructor.
+  - destruct bctx => //.
+    cbn. constructor; auto. cbn.
+    destruct (decl_body d); constructor => //. depelim p.
+    cbn in hl. assert (#|Γ| = #|bctx|) by lia.
+    rewrite map2_length //. now rewrite -H0.
+Qed.
+
+Import PCUICWeakeningEnvConv.
+
+Lemma extends_decls_trans Σ Σ' Σ'' : extends_decls Σ Σ' -> extends_decls Σ' Σ'' -> extends_decls Σ Σ''.
+Proof.
+  intros [? [ext ?]] [? [ext' ?]]. subst. split. now transitivity Σ'.
+  rewrite e0 in e2. exists (ext' ++ ext). now rewrite -app_assoc.
+Qed.
+
+Lemma declared_minductive_expanded Σ c mdecl :
+  expanded_global_env Σ ->
+  declared_minductive Σ c mdecl ->
+  exists Σ', ∥ extends_decls Σ' Σ ∥ /\ expanded_minductive_decl Σ' mdecl.
+Proof.
+  unfold expanded_global_env, declared_minductive, lookup_env.
+  destruct Σ as [univs Σ]; cbn.
+  intros exp; induction exp; cbn => //.
+  destruct decl as [kn d]; cbn.
+  destruct (eqb_spec c kn). intros [= ->].
+  subst c. eexists. split ; [|exact H]. sq. red. split => //. cbn. 
+  eexists. cbn. instantiate (1:= [_]); reflexivity.
+  intros hl; destruct (IHexp hl). exists x. intuition auto.
+  sq. eapply extends_decls_trans; tea. 
+  split => //. now exists [(kn, d)].
+Qed.
+
+Lemma declared_constructor_expanded {Σ c mdecl idecl cdecl} : 
+  expanded_global_env Σ ->
+  declared_constructor Σ c mdecl idecl cdecl ->
+  exists Σ', ∥ extends_decls Σ' Σ ∥ /\ expanded_minductive_decl Σ' mdecl /\ expanded_constructor_decl Σ' mdecl cdecl.
+Proof.
+  intros exp [[decli hnth] hnth'].
+  eapply declared_minductive_expanded in decli.
+  destruct decli as [Σ' [ext exp']]. exists Σ'; split => //. split => //.
+  destruct exp' as [hp hb]. solve_all. 
+  eapply nth_error_all in hb; tea.
+  destruct hb as [hb]. solve_all.
+  eapply nth_error_all in hb; tea.
+  auto.
+Qed.
+
+Lemma expanded_extended_subst {Σ Γ Δ} : 
+  expanded_context Σ Γ Δ -> 
+  forall n,
+  Forall (expanded Σ (repeat 0 (n + context_assumptions Δ) ++ Γ)) (extended_subst Δ n).
+Proof.
+  intros [a]; induction a. cbn. constructor.
+  cbn. destruct d as [na [b|] ty]; cbn in *. constructor; auto. 
+  { cbn. eapply (expanded_subst _ _ 0 _ []) => //. cbn. rewrite -/(repeat _ _).
+    specialize (IHa n). solve_all.
+    len. rewrite repeat_app Nat.add_comm. 
+    eapply expanded_lift. 1-2:now len; rewrite !repeat_length.
+    now depelim p. }
+  constructor; auto.
+  eapply (expanded_tRel _ _ _ _ []) => //. cbn.
+  rewrite nth_error_app_lt. rewrite repeat_length. lia.
+  rewrite nth_error_repeat //. lia.
+  specialize (IHa (S n)).
+  now rewrite Nat.add_succ_r.
+Qed.
+
+Lemma expanded_let_expansion {Σ} {Δ : context} {Γ t} :
+  expanded_context Σ Γ Δ ->
+  expanded_context Σ (repeat 0 #|Δ| ++ Γ) t ->
+  expanded_context Σ (repeat 0 (context_assumptions Δ) ++ Γ) (expand_lets_ctx Δ t).
+Proof.
+  rewrite /expanded_context.
+  intros [aΔ] [a]; sq.
+  unfold expand_lets_ctx, expand_lets_k_ctx.
+  do 2 eapply PCUICParallelReduction.All_fold_fold_context_k.
+  eapply All_fold_impl; tea. cbn.
+  intros Γ' x f. destruct (decl_body x) => //; constructor.
+  len. depelim f.
+  eapply expanded_subst. now rewrite repeat_length.
+  clear -aΔ. eapply (expanded_extended_subst (sq aΔ) 0).
+  len. rewrite app_assoc -repeat_app. eapply expanded_lift. len. now rewrite !repeat_length.
+  now rewrite repeat_length. rewrite repeat_app -app_assoc //.
+Qed.
+
+Lemma expanded_context_subst {Σ} {Δ Δ' : list nat} {Γ s k t} :
+  #|s| = #|Δ'| ->
+  #|Δ| = k ->
+  Forall (expanded Σ Γ) s ->
+  expanded_context Σ (Δ ++ repeat 0 #|Δ'| ++ Γ) t ->
+  expanded_context Σ (Δ ++ Γ) (subst_context s k t).
+Proof.
+  intros hs hs' has.
+  rewrite /expanded_context.
+  intros [aΔ]; sq.
+  eapply PCUICParallelReduction.All_fold_fold_context_k.
+  eapply All_fold_impl; tea. cbn.
+  intros Γ' x f. destruct (decl_body x) => //; constructor.
+  len. depelim f. rewrite app_assoc.
+  eapply expanded_subst. len. rewrite repeat_length. lia. solve_all. auto.
+  now rewrite -app_assoc hs.
+Qed.
+
+Lemma expanded_inds {Σ Γ ind u bodies} : Forall (expanded Σ Γ) (inds ind u bodies).
+Proof.
+  unfold inds. induction #|bodies|; cbn; auto. constructor => //. constructor.
+Qed.
+
+Implicit Types (cf : checker_flags).
+
+Lemma expanded_weakening {cf} {Σ Σ' Γ t} : 
+  wf Σ' -> extends_decls Σ Σ' -> expanded Σ Γ t -> expanded Σ' Γ t.
+Proof.
+  intros wfΣ ext.
+  eapply expanded_ind; intros.
+  all:try solve [econstructor; eauto].
+  - econstructor; eauto. solve_all. sq. eapply All_fold_impl; tea; cbn.
+    intros ? ? []; constructor; auto. now rewrite <- repeat_app.
+  - eapply expanded_tConstruct_app; tea.
+    eapply weakening_env_declared_constructor; tea. now eapply extends_decls_extends.
+Qed.
+
+Lemma expanded_context_weakening {cf} {Σ Σ' Γ t} : 
+  wf Σ' -> extends_decls Σ Σ' -> expanded_context Σ Γ t -> expanded_context Σ' Γ t.
+Proof.
+  intros wfΣ ext.
+  intros [a]; sq.
+  eapply All_fold_impl; tea; cbn; eauto.
+  intros ?? []; constructor.
+  now eapply expanded_weakening.
+Qed.
+
+Lemma expanded_bcontext {cf} Σ ind k mdecl idecl cdecl bctx bbody :
+  wf Σ ->
+  PCUICEtaExpand.expanded_global_env Σ ->
+  #|cstr_branch_context ind mdecl cdecl| = #|bctx| ->
+  declared_constructor Σ (ind, k) mdecl idecl cdecl ->
+  expanded_context Σ (repeat 0 (context_assumptions mdecl.(ind_params))) (bcontext (trans_branch ind mdecl cdecl bctx bbody)).
+Proof.
+  intros wfΣ expΣ hl declc.
+  eapply expanded_context_map2_bias_left => //.
+  destruct (declared_constructor_expanded expΣ declc) as [Σ' [ext [expm expc]]].
+  destruct expm as [hp hb]. destruct expc as [hargs hty].
+  unfold cstr_branch_context.
+  epose proof (expanded_let_expansion hp (t:=(subst_context
+  (inds (inductive_mind ind) (abstract_instance (ind_universes mdecl))
+     (ind_bodies mdecl)) #|ind_params mdecl| 
+  (cstr_args cdecl)))).
+  rewrite !app_nil_r in H. forward H.
+  epose proof (expanded_context_subst (Γ := []) (Δ' := repeat 0 #|ind_bodies mdecl|)).
+  rewrite !app_nil_r in H0. eapply H0; rewrite ?repeat_length //. len. apply expanded_inds.
+  rewrite -repeat_app. exact hargs.
+  destruct ext. eapply expanded_context_weakening; tea.
+Qed.
 
 Lemma trans_expanded {cf : checker_flags} {Σ} {wfΣ : Template.Typing.wf Σ} Γ T  :
   let Σ' := trans_global_env Σ in
   WfAst.wf Σ T ->
+  PCUICEtaExpand.expanded_global_env Σ' ->
   EtaExpand.expanded Σ Γ T ->
   expanded Σ' Γ (trans Σ' T).
 Proof with eauto using expanded.
-  intros Σ' wf exp. revert wf.
+  intros Σ' wf expΣ' exp. revert wf.
   induction exp; intros wf; cbn -[Σ']...
   all: try now (wf_inv wf []; eauto using expanded).
   - wf_inv wf ?. eapply expanded_tRel with (args := []). eauto. lia. econstructor.
@@ -41,11 +209,18 @@ Proof with eauto using expanded.
     erewrite trans_lookup_inductive, declared_inductive_lookup; eauto.
     econstructor; eauto. cbn.
     + solve_all.
-    + cbn. induction a1; cbn; econstructor.
-      * split.
-        sq. cbn.
-      cbn. inversion H0; subst. rewrite map2_bias_left_length. len. eapply H3. eapply r.
-    + inversion H0; subst. inversion H; subst. eapply IHa1; eauto.
+    + cbn. eapply All2_nth_hyp in a1.
+      eapply All_Forall, All2_All_map2, All2_map.
+      eapply Forall_All in H2. eapply All2_All_mix_right in a1; tea.
+      eapply All2_impl; tea. intros x y. cbv beta. intros [[i [Hi []]] ?].
+      split.
+      { rewrite map_length. relativize #|Ast.pparams type_info|.
+        eapply expanded_bcontext => //.
+        - now eapply template_to_pcuic_env.
+        - len. eapply All2_length in a2. len in a2.
+        - split; tea. cbn; rewrite nth_error_map. erewrite Hi => //.
+        - cbn. tea. rewrite context_assumptions_map. now rewrite e. }
+      * cbn. rewrite map2_bias_left_length. now eapply e0.
     + eapply template_to_pcuic_env; eauto.
   - now (wf_inv wf [[]]; eauto using expanded).
   - wf_inv wf [[]]. wf_inv w ?. eapply expanded_tFix.
